@prefix sc:    <http://shapechange.net/resources/ont/base#> .
@prefix core:  <https://github.com/VCityTeam/UD-Graph/Ontologies/core#> .
@prefix gen:   <https://github.com/VCityTeam/UD-Graph/Ontologies/generics#> .
@prefix iso19150-2: <http://def.isotc211.org/iso19150/-2/2012/base#> .
@prefix rdf:   <http://www.w3.org/1999/02/22-rdf-syntax-ns#> .
@prefix owl:   <http://www.w3.org/2002/07/owl#> .
@prefix xsd:   <http://www.w3.org/2001/XMLSchema#> .
@prefix skos:  <http://www.w3.org/2004/02/skos/core#> .
@prefix rdfs:  <http://www.w3.org/2000/01/rdf-schema#> .

gen:CodeAttribute.value
        a                owl:ObjectProperty ;
        rdfs:domain      gen:CodeAttribute ;
        rdfs:range       core:Code ;
        skos:definition  "Specifies the \"Code\" value."@en ;
        skos:prefLabel   "value"@en .

gen:GenericUnoccupiedSpace.function
        a                owl:ObjectProperty ;
        rdfs:domain      gen:GenericUnoccupiedSpace ;
        rdfs:range       gen:GenericUnoccupiedSpaceFunctionValue ;
        skos:definition  "Specifies the intended purposes of the GenericUnoccupiedSpace."@en ;
        skos:prefLabel   "function"@en .

gen:GenericUnoccupiedSpaceUsageValue
        a                owl:Class ;
        rdfs:subClassOf  skos:Concept ;
        skos:definition  "GenericUnoccupiedSpaceUsageValue is a code list that enumerates the different uses of a GenericUnoccupiedSpace."@en ;
        skos:prefLabel   "GenericUnoccupiedSpaceUsageValue"@en .

gen:GenericAttributeSet
        a                owl:Class ;
        rdfs:subClassOf  core:AbstractGenericAttribute ;
        skos:definition  "A GenericAttributeSet is a named collection of generic attributes."@en ;
        skos:prefLabel   "GenericAttributeSet"@en .

gen:CodeAttribute.name
        a                owl:DatatypeProperty ;
        rdfs:domain      gen:CodeAttribute ;
        rdfs:range       xsd:string ;
        skos:definition  "Specifies the name of the CodeAttribute."@en ;
        skos:prefLabel   "name"@en .

gen:GenericThematicSurfaceFunctionValue
        a                owl:Class ;
        rdfs:subClassOf  skos:Concept ;
        skos:definition  "GenericThematicSurfaceFunctionValue is a code list that enumerates the different purposes of a GenericThematicSurface."@en ;
        skos:prefLabel   "GenericThematicSurfaceFunctionValue"@en .

gen:ADEOfGenericUnoccupiedSpace
        a                      owl:Class ;
        iso19150-2:isAbstract  true ;
        skos:definition        "ADEOfGenericUnoccupiedSpace acts as a hook to define properties within an ADE that are to be added to a GenericUnoccupiedSpace."@en ;
        skos:prefLabel         "ADEOfGenericUnoccupiedSpace"@en .

gen:GenericOccupiedSpace.usage
        a                owl:ObjectProperty ;
        rdfs:domain      gen:GenericOccupiedSpace ;
        rdfs:range       gen:GenericOccupiedSpaceUsageValue ;
        skos:definition  "Specifies the actual uses of the GenericOccupiedSpace."@en ;
        skos:prefLabel   "usage"@en .

gen:GenericThematicSurface.adeOfGenericThematicSurface
        a                owl:ObjectProperty ;
        rdfs:domain      gen:GenericThematicSurface ;
        rdfs:range       gen:ADEOfGenericThematicSurface ;
        skos:definition  "Augments the GenericThematicSurface with properties defined in an ADE."@en ;
        skos:prefLabel   "adeOfGenericThematicSurface"@en .

gen:GenericOccupiedSpaceUsageValue
        a                owl:Class ;
        rdfs:subClassOf  skos:Concept ;
        skos:definition  "GenericOccupiedSpaceUsageValue is a code list that enumerates the different uses of a GenericOccupiedSpace."@en ;
        skos:prefLabel   "GenericOccupiedSpaceUsageValue"@en .

gen:GenericAttributeSet.genericAttribute
        a                owl:ObjectProperty ;
        rdfs:domain      gen:GenericAttributeSet ;
        rdfs:range       core:AbstractGenericAttribute ;
        skos:definition  "Relates to the generic attributes that are part of the GenericAttributeSet."@en ;
        skos:prefLabel   "genericAttribute"@en .

gen:GenericOccupiedSpaceFunctionValue
        a                owl:Class ;
        rdfs:subClassOf  skos:Concept ;
        skos:definition  "GenericOccupiedSpaceFunctionValue is a code list that enumerates the different purposes of a GenericOccupiedSpace."@en ;
        skos:prefLabel   "GenericOccupiedSpaceFunctionValue"@en .

gen:DateAttribute  a     owl:Class ;
        rdfs:subClassOf  core:AbstractGenericAttribute ;
        skos:definition  "DateAttribute is a data type used to define generic attributes of type \"Date\"."@en ;
        skos:prefLabel   "DateAttribute"@en .

gen:GenericLogicalSpaceUsageValue
        a                owl:Class ;
        rdfs:subClassOf  skos:Concept ;
        skos:definition  "GenericLogicalSpaceUsageValue is a code list that enumerates the different uses of a GenericLogicalSpace."@en ;
        skos:prefLabel   "GenericLogicalSpaceUsageValue"@en .

gen:CodeAttribute  a     owl:Class ;
        rdfs:subClassOf  core:AbstractGenericAttribute ;
        skos:definition  "CodeAttribute is a data type used to define generic attributes of type \"Code\"."@en ;
        skos:prefLabel   "CodeAttribute"@en .

gen:GenericUnoccupiedSpace.class
        a                owl:ObjectProperty ;
        rdfs:domain      gen:GenericUnoccupiedSpace ;
        rdfs:range       gen:GenericUnoccupiedSpaceClassValue ;
        skos:definition  "Indicates the specific type of the GenericUnoccupiedSpace."@en ;
        skos:prefLabel   "class"@en .

gen:ADEOfGenericOccupiedSpace
        a                      owl:Class ;
        iso19150-2:isAbstract  true ;
        skos:definition        "ADEOfGenericOccupiedSpace acts as a hook to define properties within an ADE that are to be added to a GenericOccupiedSpace."@en ;
        skos:prefLabel         "ADEOfGenericOccupiedSpace"@en .

gen:GenericThematicSurface.usage
        a                owl:ObjectProperty ;
        rdfs:domain      gen:GenericThematicSurface ;
        rdfs:range       gen:GenericThematicSurfaceUsageValue ;
        skos:definition  "Specifies the actual uses of the GenericThematicSurface."@en ;
        skos:prefLabel   "usage"@en .

gen:UriAttribute  a      owl:Class ;
        rdfs:subClassOf  core:AbstractGenericAttribute ;
        skos:definition  "UriAttribute is a data type used to define generic attributes of type \"URI\"."@en ;
        skos:prefLabel   "UriAttribute"@en .

gen:GenericUnoccupiedSpace
        a                owl:Class ;
        rdfs:subClassOf  core:AbstractUnoccupiedSpace ;
        skos:definition  "A GenericUnoccupiedSpace is a space that is not represented by any explicitly modelled AbstractUnoccupiedSpace subclass within CityGML."@en ;
        skos:prefLabel   "GenericUnoccupiedSpace"@en .

gen:MeasureAttribute.name
        a                owl:DatatypeProperty ;
        rdfs:domain      gen:MeasureAttribute ;
        rdfs:range       xsd:string ;
        skos:definition  "Specifies the name of the MeasureAttribute."@en ;
        skos:prefLabel   "name"@en .

gen:StringAttribute.name
        a                owl:DatatypeProperty ;
        rdfs:domain      gen:StringAttribute ;
        rdfs:range       xsd:string ;
        skos:definition  "Specifies the name of the StringAttribute."@en ;
        skos:prefLabel   "name"@en .

gen:GenericLogicalSpace.adeOfGenericLogicalSpace
        a                owl:ObjectProperty ;
        rdfs:domain      gen:GenericLogicalSpace ;
        rdfs:range       gen:ADEOfGenericLogicalSpace ;
        skos:definition  "Augments the GenericLogicalSpace with properties defined in an ADE."@en ;
        skos:prefLabel   "adeOfGenericLogicalSpace"@en .

gen:MeasureAttribute  a  owl:Class ;
        rdfs:subClassOf  core:AbstractGenericAttribute ;
        skos:definition  "MeasureAttribute is a data type used to define generic attributes of type \"Measure\"."@en ;
        skos:prefLabel   "MeasureAttribute"@en .

gen:IntAttribute.value
        a                owl:DatatypeProperty ;
        rdfs:domain      gen:IntAttribute ;
        rdfs:range       xsd:integer ;
        skos:definition  "Specifies the \"Integer\" value."@en ;
        skos:prefLabel   "value"@en .

gen:DateAttribute.value
        a                owl:DatatypeProperty ;
        rdfs:domain      gen:DateAttribute ;
        rdfs:range       xsd:date ;
        skos:definition  "Specifies the \"Date\" value."@en ;
        skos:prefLabel   "value"@en .

gen:UriAttribute.value
        a                owl:DatatypeProperty ;
        rdfs:domain      gen:UriAttribute ;
        rdfs:range       xsd:anyURI ;
        skos:definition  "Specifies the \"URI\" value."@en ;
        skos:prefLabel   "value"@en .

<https://github.com/VCityTeam/UD-Graph/Ontologies/generics>
        a                owl:Ontology ;
        owl:imports      <http://shapechange.net/resources/ont/base> , <https://github.com/VCityTeam/UD-Graph/Ontologies/core> , <http://def.isotc211.org/iso19150/-2/2012/base> ;
        owl:versionIRI   "https://github.com/VCityTeam/UD-Graph/Ontologies/generics/3.0.0" ;
        owl:versionInfo  "3.0.0" ;
        skos:definition  "The Generics module supports application-specific extensions to the CityGML data model. These extensions may be used to model and exchange additional attributes and features not covered by the predefined thematic classes of CityGML. Generic extensions shall only be used if appropriate thematic classes or attributes are not provided by any other CityGML module."@en ;
        skos:prefLabel   "Generics"@en .

gen:GenericAttributeSet.codeSpace
        a                owl:DatatypeProperty ;
        rdfs:domain      gen:GenericAttributeSet ;
        rdfs:range       xsd:anyURI ;
        skos:definition  "Associates the GenericAttributeSet with an authority that maintains the collection of generic attributes."@en ;
        skos:prefLabel   "codeSpace"@en .

gen:DateAttribute.name
        a                owl:DatatypeProperty ;
        rdfs:domain      gen:DateAttribute ;
        rdfs:range       xsd:string ;
        skos:definition  "Specifies the name of the DateAttribute."@en ;
        skos:prefLabel   "name"@en .

gen:GenericUnoccupiedSpace.usage
        a                owl:ObjectProperty ;
        rdfs:domain      gen:GenericUnoccupiedSpace ;
        rdfs:range       gen:GenericUnoccupiedSpaceUsageValue ;
        skos:definition  "Specifies the actual uses of the GenericUnoccupiedSpace."@en ;
        skos:prefLabel   "usage"@en .

gen:GenericLogicalSpaceFunctionValue
        a                owl:Class ;
        rdfs:subClassOf  skos:Concept ;
        skos:definition  "GenericLogicalSpaceFunctionValue is a code list that enumerates the different purposes of a GenericLogicalSpace."@en ;
        skos:prefLabel   "GenericLogicalSpaceFunctionValue"@en .

gen:GenericLogicalSpace.class
        a                owl:ObjectProperty ;
        rdfs:domain      gen:GenericLogicalSpace ;
        rdfs:range       gen:GenericLogicalSpaceClassValue ;
        skos:definition  "Indicates the specific type of the GenericLogicalSpace."@en ;
        skos:prefLabel   "class"@en .

gen:UriAttribute.name
        a                owl:DatatypeProperty ;
        rdfs:domain      gen:UriAttribute ;
        rdfs:range       xsd:string ;
        skos:definition  "Specifies the name of the UriAttribute."@en ;
        skos:prefLabel   "name"@en .

gen:GenericUnoccupiedSpaceClassValue
        a                owl:Class ;
        rdfs:subClassOf  skos:Concept ;
        skos:definition  "GenericUnoccupiedSpaceClassValue is a code list used to further classify a GenericUnoccupiedSpace."@en ;
        skos:prefLabel   "GenericUnoccupiedSpaceClassValue"@en .

gen:DoubleAttribute.name
        a                owl:DatatypeProperty ;
        rdfs:domain      gen:DoubleAttribute ;
        rdfs:range       xsd:string ;
        skos:definition  "Specifies the name of the DoubleAttribute."@en ;
        skos:prefLabel   "name"@en .

gen:StringAttribute  a   owl:Class ;
        rdfs:subClassOf  core:AbstractGenericAttribute ;
        skos:definition  "StringAttribute is a data type used to define generic attributes of type \"String\"."@en ;
        skos:prefLabel   "StringAttribute"@en .

gen:GenericOccupiedSpace
        a                owl:Class ;
        rdfs:subClassOf  core:AbstractOccupiedSpace ;
        skos:definition  "A GenericOccupiedSpace is a space that is not represented by any explicitly modelled AbstractOccupiedSpace subclass within CityGML."@en ;
        skos:prefLabel   "GenericOccupiedSpace"@en .

gen:GenericAttributeSet.name
        a                owl:DatatypeProperty ;
        rdfs:domain      gen:GenericAttributeSet ;
        rdfs:range       xsd:string ;
        skos:definition  "Specifies the name of the GenericAttributeSet."@en ;
        skos:prefLabel   "name"@en .

gen:ADEOfGenericThematicSurface
        a                      owl:Class ;
        iso19150-2:isAbstract  true ;
        skos:definition        "ADEOfGenericThematicSurface acts as a hook to define properties within an ADE that are to be added to a GenericThematicSurface."@en ;
        skos:prefLabel         "ADEOfGenericThematicSurface"@en .

gen:GenericThematicSurfaceClassValue
        a                owl:Class ;
        rdfs:subClassOf  skos:Concept ;
        skos:definition  "GenericThematicSurfaceClassValue is a code list used to further classify a GenericThematicSurface."@en ;
        skos:prefLabel   "GenericThematicSurfaceClassValue"@en .

gen:GenericUnoccupiedSpace.adeOfGenericUnoccupiedSpace
        a                owl:ObjectProperty ;
        rdfs:domain      gen:GenericUnoccupiedSpace ;
        rdfs:range       gen:ADEOfGenericUnoccupiedSpace ;
        skos:definition  "Augments the GenericUnoccupiedSpace with properties defined in an ADE."@en ;
        skos:prefLabel   "adeOfGenericUnoccupiedSpace"@en .

gen:GenericUnoccupiedSpaceFunctionValue
        a                owl:Class ;
        rdfs:subClassOf  skos:Concept ;
        skos:definition  "GenericUnoccupiedSpaceFunctionValue is a code list that enumerates the different purposes of a GenericUnoccupiedSpace."@en ;
        skos:prefLabel   "GenericUnoccupiedSpaceFunctionValue"@en .

gen:GenericThematicSurface.function
        a                owl:ObjectProperty ;
        rdfs:domain      gen:GenericThematicSurface ;
        rdfs:range       gen:GenericThematicSurfaceFunctionValue ;
        skos:definition  "Specifies the intended purposes of the GenericThematicSurface."@en ;
        skos:prefLabel   "function"@en .

gen:MeasureAttribute.value
        a                owl:DatatypeProperty ;
        rdfs:domain      gen:MeasureAttribute ;
        rdfs:range       sc:Measure ;
        skos:definition  "Specifies the value of the MeasureAttribute. The value is of type \"Measure\", which can additionally provide the units of measure. [cf. ISO 19103]"@en ;
        skos:prefLabel   "value"@en .

gen:IntAttribute  a      owl:Class ;
        rdfs:subClassOf  core:AbstractGenericAttribute ;
        skos:definition  "IntAttribute is a data type used to define generic attributes of type \"Integer\"."@en ;
        skos:prefLabel   "IntAttribute"@en .

gen:GenericLogicalSpace.function
        a                owl:ObjectProperty ;
        rdfs:domain      gen:GenericLogicalSpace ;
        rdfs:range       gen:GenericLogicalSpaceFunctionValue ;
        skos:definition  "Specifies the intended purposes of the GenericLogicalSpace."@en ;
        skos:prefLabel   "function"@en .

gen:IntAttribute.name
        a                owl:DatatypeProperty ;
        rdfs:domain      gen:IntAttribute ;
        rdfs:range       xsd:string ;
        skos:definition  "Specifies the name of the IntAttribute."@en ;
        skos:prefLabel   "name"@en .

gen:ADEOfGenericLogicalSpace
        a                      owl:Class ;
        iso19150-2:isAbstract  true ;
        skos:definition        "ADEOfGenericLogicalSpace acts as a hook to define properties within an ADE that are to be added to a GenericLogicalSpace."@en ;
        skos:prefLabel         "ADEOfGenericLogicalSpace"@en .

gen:GenericLogicalSpace.usage
        a                owl:ObjectProperty ;
        rdfs:domain      gen:GenericLogicalSpace ;
        rdfs:range       gen:GenericLogicalSpaceUsageValue ;
        skos:definition  "Specifies the actual uses of the GenericLogicalSpace."@en ;
        skos:prefLabel   "usage"@en .

gen:GenericOccupiedSpace.class
        a                owl:ObjectProperty ;
        rdfs:domain      gen:GenericOccupiedSpace ;
        rdfs:range       gen:GenericOccupiedSpaceClassValue ;
        skos:definition  "Indicates the specific type of the GenericOccupiedSpace."@en ;
        skos:prefLabel   "class"@en .

gen:GenericThematicSurface
        a                owl:Class ;
        rdfs:subClassOf  core:AbstractThematicSurface ;
        skos:definition  "A GenericThematicSurface is a surface that is not represented by any explicitly modelled AbstractThematicSurface subclass within CityGML."@en ;
        skos:prefLabel   "GenericThematicSurface"@en .

gen:GenericLogicalSpace
        a                owl:Class ;
        rdfs:subClassOf  core:AbstractLogicalSpace ;
        skos:definition  "A GenericLogicalSpace is a space that is not represented by any explicitly modelled AbstractLogicalSpace subclass within CityGML."@en ;
        skos:prefLabel   "GenericLogicalSpace"@en .

gen:DoubleAttribute.value
        a                owl:DatatypeProperty ;
        rdfs:domain      gen:DoubleAttribute ;
        rdfs:range       xsd:double ;
        skos:definition  "Specifies the \"Double\" value."@en ;
        skos:prefLabel   "value"@en .

gen:GenericOccupiedSpace.function
        a                owl:ObjectProperty ;
        rdfs:domain      gen:GenericOccupiedSpace ;
        rdfs:range       gen:GenericOccupiedSpaceFunctionValue ;
        skos:definition  "Specifies the intended purposes of the GenericOccupiedSpace."@en ;
        skos:prefLabel   "function"@en .

gen:GenericThematicSurfaceUsageValue
        a                owl:Class ;
        rdfs:subClassOf  skos:Concept ;
        skos:definition  "GenericThematicSurfaceUsageValue is a code list that enumerates the different uses of a GenericThematicSurface."@en ;
        skos:prefLabel   "GenericThematicSurfaceUsageValue"@en .

gen:StringAttribute.value
        a                owl:DatatypeProperty ;
        rdfs:domain      gen:StringAttribute ;
        rdfs:range       xsd:string ;
        skos:definition  "Specifies the \"String\" value."@en ;
        skos:prefLabel   "value"@en .

gen:GenericThematicSurface.class
        a                owl:ObjectProperty ;
        rdfs:domain      gen:GenericThematicSurface ;
        rdfs:range       gen:GenericThematicSurfaceClassValue ;
        skos:definition  "Indicates the specific type of the GenericThematicSurface."@en ;
        skos:prefLabel   "class"@en .

gen:DoubleAttribute  a   owl:Class ;
        rdfs:subClassOf  core:AbstractGenericAttribute ;
        skos:definition  "DoubleAttribute is a data type used to define generic attributes of type \"Double\"."@en ;
        skos:prefLabel   "DoubleAttribute"@en .

gen:GenericOccupiedSpaceClassValue
        a                owl:Class ;
        rdfs:subClassOf  skos:Concept ;
        skos:definition  "GenericOccupiedSpaceClassValue is a code list used to further classify a GenericOccupiedSpace."@en ;
        skos:prefLabel   "GenericOccupiedSpaceClassValue"@en .

gen:GenericOccupiedSpace.adeOfGenericOccupiedSpace
        a                owl:ObjectProperty ;
        rdfs:domain      gen:GenericOccupiedSpace ;
        rdfs:range       gen:ADEOfGenericOccupiedSpace ;
        skos:definition  "Augments the GenericOccupiedSpace with properties defined in an ADE."@en ;
        skos:prefLabel   "adeOfGenericOccupiedSpace"@en .

gen:GenericLogicalSpaceClassValue
        a                owl:Class ;
        rdfs:subClassOf  skos:Concept ;
        skos:definition  "GenericLogicalSpaceClassValue is a code list used to further classify a GenericLogicalSpace."@en ;
        skos:prefLabel   "GenericLogicalSpaceClassValue"@en .
